src/tosmt/term.fsi
@@ -153,6 +153,7 @@ val mk_ApplyTT: term -> term -> term
 val mk_ApplyET: term -> term -> term
 val mk_ApplyEE: term -> term -> term
 val mk_String_const: int -> term
-
+val mk_Precedes: term -> term -> term
+val mk_LexPair: term -> term -> term
 val freeV_sym: term -> string
 val boundV_sym:term -> string
