examples/unit-tests/listlemmas.fst
@@ -16,12 +16,7 @@
 
 
 (*
-   TODO: Termination checking is not yet implemented. 
-  
-   A let rec with an explicitly annotated "Tot" effect is admitted. 
-   Without such an annotation, the inferred effect is "All" 
-
-   Termination checks to be added soon ... 
+   Termination checking is ON
 *)
 
 module ListLemmas
@@ -37,7 +32,7 @@ let rec zero l = match l with
   | [] -> 0
   | hd::tl -> zero tl
 
-(* Using a refinement type to prove a property of a function as it is being defined, 
+(* Using a refinement type to prove a property of a function as it is being defined,
    i.e., an intrinsic proof about length being non-negative *)
 val length: list 'a -> Tot nat
 let rec length l = match l with
@@ -51,7 +46,7 @@ let rec mem a l = match l with
   | hd::tl -> hd=a || mem a tl
 
 (* Prove a property about the length of appended lists intrinsically.
-   Notice the use of the pure function length in the spec. 
+   Notice the use of the pure function length in the spec.
  *)
 val append: l1:list 'a -> l2:list 'a -> Tot (l3:list 'a{length l3 == length l1 + length l2})
 let rec append l1 l2 =  match l1 with
@@ -64,7 +59,7 @@ For contrast, in old F*/F7, you'd have to write:
    assume Length_nil: ...
    assume Length_cons: ...
    val length: l:list 'a -> (n:nat{n=Length l})
-   let rec length l = ... 
+   let rec length l = ...
 
    val append: l1:list 'a -> l2:list 'a -> (l3:list 'a{Length l3 = Length l1 + Length l2})
    let rec append = ...
@@ -72,8 +67,8 @@ For contrast, in old F*/F7, you'd have to write:
 
 assume val ignore: unit -> Fact unit False
 
-(* You can also prove lemmas about pure functions "after the fact", i.e., extrinsically. 
-   Here's an inductive proofs relating append and mem. 
+(* You can also prove lemmas about pure functions "after the fact", i.e., extrinsically.
+   Here's an inductive proofs relating append and mem.
 
    Note also the use of boolean valued terms as predicates. I'm
    beginning to add support for automatically lifting bool to Type,
@@ -85,17 +80,17 @@ val append_mem:  l1:list 'a
               -> Fact unit (ensures (mem a (append l1 l2) <==>  mem a l1 \/ mem a l2))
 let rec append_mem l1 l2 a = match l1 with
   | [] -> ()
-  | hd::tl -> 
+  | hd::tl ->
     if hd=a
     then ()
     else append_mem tl l2 a
   
-(*   
+(*
    Such an extrinsic proof would have been impossible in old F*/F7. You'd have to
    prove the relation between mem and append intrinsically.
 
-   Alternatively, you could 
-     1. define a logic function Append and Mem (like Length above), 
+   Alternatively, you could
+     1. define a logic function Append and Mem (like Length above),
      2. intrinsically prove the connection between append and Append, mem and Mem
      3. extrinsically try to use induction to prove relate Append and Mem
 
@@ -116,7 +111,7 @@ let rec map f l = match l with
 let plus_one x = x + 1
 
 val test_map: unit -> Tot unit
-let test_map x = 
+let test_map x =
   let l = [0;1;2] in
   let g = map plus_one l in
   assert (g == [1;2;3])
